src/cbor/pulse/raw/CBOR.Pulse.Raw.Format.Serialized.Iterator.fsti
@@ -1,7 +1,0 @@
-module CBOR.Pulse.Raw.Format.Serialized.Iterator
-
-[@@CAbstractStruct]
-val cbor_serialized_array_iterator: Type0
-
-[@@CAbstractStruct]
-val cbor_serialized_map_iterator: Type0
