src/cbor/pulse/raw/CBOR.Pulse.Raw.Iterator.Base.fst
@@ -1,0 +1,9 @@
+module CBOR.Pulse.Raw.Iterator.Base
+module S = Pulse.Lib.Slice
+module U8 = FStar.UInt8
+
+noeq
+type cbor_raw_serialized_iterator = {
+  s: S.slice U8.t;
+  len: Ghost.erased nat;
+}
