src/cbor/pulse/raw/everparse/CBOR.Pulse.Raw.Format.Serialized.Iterator.fst
@@ -1,7 +1,0 @@
-module CBOR.Pulse.Raw.Format.Serialized.Iterator
-open CBOR.Pulse.Raw.EverParse.Iterator
-
-let cbor_serialized_array_iterator = cbor_raw_serialized_iterator 
-
-let cbor_serialized_map_iterator = cbor_raw_serialized_iterator 
-
